Add first ideas for monad actions

test-suite/monads.v
@@ -1,11 +1,42 @@
-Require Import List.
+Declare ML Module "paramcoq".
 
-Module MaybeMonad.
+Require Import List.
+(* Require Import Basics. *)
+
+(* Print flip. *)
+
+Set Implicit Arguments.
+
+Print flat_map.
+Definition flip {A B C} (f : A -> B -> C) x y : C := f y x.
+
+Print flip.
+
+Section MonadClass.
+
+  Class Monad (M : Type -> Type) := {
+  bind : forall A B,
+    M A -> (A -> M B) -> M B;
+  unit : forall A , A -> M A;
+  bind_assoc :
+    forall A B C
+    (m : M A)
+    (f : A -> M B) (g : B -> M C),
+    bind (bind m f) g = bind m (fun i => bind (f i) g);
+  right_unit : forall A (m : M A),
+    bind m (@unit A) = m;
+  left_unit : forall A B (x : A) (f : A -> M B),
+    bind (unit x) f = f x
+}.
+
+Section MonadClass.
+
+
+Section MaybeMonad.
 
   Inductive option (A : Type) :=
   | Some : A -> option A
   | None : option A.
-
 
   (* Without Implicit Arguments *)
 
@@ -19,48 +50,57 @@ Module MaybeMonad.
   Arguments Some {A} _.
   Arguments None {A}.
 
-  Definition ret {A: Type} (x : A) := Some x.
-  Definition bind {A B : Type} (a : option A) (f: A -> option B) : option B :=
+  Definition option_ret {A: Type} (x : A) := Some x.
+  Definition option_bind {A B : Type} (a : option A) (f: A -> option B) : option B :=
     match a with
       | Some x => f x
       | None => None
     end.
 
-  Lemma monad_left_identity :
-    forall (A B : Type) (x : A) (f : A -> option B), bind (ret x) f = f x.
+  Lemma option_left_identity :
+    forall (A B : Type) (x : A) (f : A -> option B), option_bind (option_ret x) f = f x.
     repeat intro.
     compute.
     trivial.
   Qed.
 
-  Lemma monad_right_identity :
-    forall (A B : Type) (mx : option A), bind mx ret = mx.
+  Lemma option_right_identity :
+    forall (A : Type) (mx : option A), option_bind mx option_ret = mx.
     repeat intro.
     induction mx; compute; reflexivity.
   Qed.
 
-  Lemma monad_associativity :
+  Lemma option_associativity :
     forall (A B C : Type) (mx : option A) (f : A -> option B) (g : B -> option C),
-      bind (bind mx f) g = bind mx (fun x => bind (f x) g).
+      option_bind (option_bind mx f) g = option_bind mx (fun x => option_bind (f x) g).
     repeat intro.
     induction mx; compute.
     induction (f a); trivial.
     trivial.
   Qed.
 
+  Instance option_monad : Monad option :=
+    {
+      bind := fun X => fun Y => option_bind;
+      unit := fun X => option_ret;
+      bind_assoc := option_associativity;
+      left_unit := option_left_identity;
+      right_unit := option_right_identity
+    }. 
+
 End MaybeMonad.
 
-Module ListMonad.
+Section ListMonad.
 
   (* Inductive list (A : Type) := *)
   (* | cons : A -> list A -> list A*)
   (* | nil : list A. *)
 
-  Arguments nil {A}.
-  Arguments cons {A} _ _.
+  (* Arguments nil {A}. *)
+  (* Arguments cons {A} _ _. *)
 
-  Definition ret {A : Type} (x : A) := cons x nil.
-  Definition bind {A B : Type} (mx : list A) (f : A -> list B) : list B :=
+  Definition list_ret {A : Type} (x : A) := cons x nil.
+  Definition list_bind {A B : Type} (mx : list A) (f : A -> list B) : list B :=
     flat_map f mx.
 
   (* Fixpoint bind {A B : Type} (mx : list A) (f : A -> list B) : list B := *)
@@ -69,19 +109,19 @@ Module ListMonad.
   (*     | cons x my => f x ++ bind my f  * *)
   (*   end. *)
   
-  Lemma monad_left_identity :
-    forall (A B : Type) (x : A) (f : A -> list B), bind (ret x) f = f x.
+  Lemma list_left_identity :
+    forall (A B: Type) (x : A) (f : A -> list B), list_bind (list_ret x) f = f x.
     repeat intro.
-    unfold ret.
-    unfold bind.
+    unfold list_ret.
+    unfold list_bind.
     unfold flat_map.
     SearchAbout nil.
     rewrite  (app_nil_r (f x)).
     reflexivity.
   Qed.
 
-  Lemma monad_right_identity :
-    forall (A B : Type) (mx : list A), bind mx ret = mx.
+  Lemma list_right_identity :
+    forall (A : Type) (mx : list A), list_bind mx list_ret = mx.
     repeat intro.
     induction mx.
     compute; trivial.
@@ -102,14 +142,51 @@ Qed.
     apply app_assoc.
   Qed.
   
-  Lemma monad_associativity :
+  Lemma list_associativity :
     forall (A B C : Type) (mx : list A) (f : A -> list B) (g : B -> list C),
-      bind (bind mx f) g = bind mx (fun x => bind (f x) g).
+      list_bind (list_bind mx f) g = list_bind mx (fun x => list_bind (f x) g).
     repeat intro.
     induction mx; simpl.
     trivial.
     rewrite <- IHmx.
     apply flat_map_app.
   Qed.
+
+  Print flip.
+  Print flat_map.
+
+  Instance list_monad : Monad list :=
+    {
+      bind := fun X => fun Y => list_bind;
+      unit := fun X => list_ret;
+      bind_assoc := list_associativity;
+      left_unit := list_left_identity;
+      right_unit := list_right_identity
+    }. 
   
 End ListMonad.
+
+Section MonadAction.
+
+
+  (* Definition in_relation (A B : Type) := forall (x : A) (y : B), Prop. *)
+
+  (* Inductive Rel : Type := *)
+  (*   | EmbedRel : forall S T, in_relation S T -> Rel. *)
+
+  (* Definition full_relation {A B} (t1 : A) (t2 : B) := True. *)
+  (* Print Monad. *)
+  (* Definition function_relation {A B M1 M2} *)
+  (*            (Rel : A -> B -> Prop) (t1 : A -> Monad (M1 A)) (t2 : B -> Monad (M2 B)) *)
+  (*            : Prop := forall x y, Rel x y -> full_relation (t1 x) (t2 y). *)
+  (* Definition F {A B : Set} (R : Type) (k1 : A) (k2 : B) : Type := *)
+  (*  forall Tau1 Tau2, (Parametricity R) /\ R_R Tau1 Tau2.  *)
+  (* Definition Monad_Action {A B X Y} (k1 : Monad A) (k2 : Monad B) : Type := *)
+  (*   function_relation full_relation (unit : X -> k1) (unit). *)
+
+  (* Print full_relation. *)
+  (* Definition Maybe_List_FR {A B} (R : A -> B -> Prop) := *)
+  (*   full_relation (None A) (nil : list B) /\ *)
+  (*   function_relation R (fun x => Some x) (fun z => cons z nil). *)
+  
+End MonadAction.
